prove "THE CLIENT"

barrier/client.v
@@ -2,21 +2,69 @@ From barrier Require Import proof.
 From program_logic Require Import auth sts saved_prop hoare ownership.
 Import uPred.
 
-Definition client := (let: "b" := newbarrier '() in wait "b")%L.
+Definition worker (n : Z) := (λ: "b" "y", wait "b" ;; (!"y") 'n)%L.
+Definition client := (let: "y" := ref '0 in let: "b" := newbarrier '() in
+                      Fork (Skip ;; Fork (worker 12 "b" "y") ;; worker 17 "b" "y") ;;
+                      "y" <- (λ: "z", "z" + '42) ;; signal "b")%L.
 
 Section client.
   Context {Σ : iFunctorG} `{!heapG Σ, !barrierG Σ} (heapN N : namespace).
   Local Notation iProp := (iPropG heap_lang Σ).
 
+  Definition y_inv q y : iProp := (∃ f : val, y ↦{q} f ★ □ ∀ n : Z,
+                            (* TODO: '() conflicts with '(n + 42)... *)
+                            || f 'n {{ λ v, v = LitV (n + 42)%Z }})%I.
+  
+  Lemma y_inv_split q y :
+    y_inv q y ⊑ (y_inv (q/2) y ★ y_inv (q/2) y).
+  Proof.
+    rewrite /y_inv. apply exist_elim=>f.
+    rewrite -!(exist_intro f). rewrite heap_mapsto_op_split.
+    ecancel [y ↦{_} _; y ↦{_} _]%I. by rewrite [X in X ⊑ _]always_sep_dup.
+  Qed.
+
+  Lemma worker_safe q (n : Z) (b y : loc) :
+    (heap_ctx heapN ★ recv heapN N b (y_inv q y))
+      ⊑ || worker n (Loc b) (Loc y) {{ λ _, True }}.
+  Proof.
+    rewrite /worker. wp_lam. wp_let. ewp apply wait_spec.
+    rewrite comm. apply sep_mono_r. apply wand_intro_l.
+    rewrite sep_exist_r. apply exist_elim=>f. wp_seq.
+    (* TODO these aprenthesis are rather surprising. *)
+    (ewp apply: (wp_load heapN _ _ q f)); eauto with I.
+    strip_later. (* hu, shouldn't it do that? *)
+    rewrite -assoc. apply sep_mono_r. apply wand_intro_l.
+    rewrite always_elim (forall_elim n) sep_elim_r sep_elim_l.
+    apply wp_mono=>?. eauto with I.
+  Qed.
+
   Lemma client_safe :
     heapN ⊥ N → heap_ctx heapN ⊑ || client {{ λ _, True }}.
   Proof.
     intros ?. rewrite /client.
-    ewp eapply (newbarrier_spec heapN N True%I); last done.
-    apply sep_intro_True_r; first done.
-    apply forall_intro=>l. apply wand_intro_l. rewrite right_id.
-    wp_let. etrans; last eapply wait_spec.
-    apply sep_mono_r, wand_intro_r. eauto.
+    (ewp eapply wp_alloc); eauto with I. strip_later. apply forall_intro=>y.
+    apply wand_intro_l. wp_let.
+    ewp eapply (newbarrier_spec heapN N (y_inv 1 y)); last done.
+    rewrite comm. rewrite {1}[heap_ctx _]always_sep_dup -!assoc.
+    apply sep_mono_r. apply forall_intro=>b. apply wand_intro_l. 
+    wp_let. ewp eapply wp_fork.
+    rewrite [heap_ctx _]always_sep_dup !assoc [(_ ★ heap_ctx _)%I]comm.
+    rewrite [(|| _ {{ _ }} ★ _)%I]comm -!assoc assoc. apply sep_mono;last first.
+    { (* The original thread, the sender. *)
+      wp_seq. (ewp eapply wp_store); eauto with I. strip_later.
+      rewrite assoc [(_ ★ y ↦ _)%I]comm. apply sep_mono_r, wand_intro_l.
+      wp_seq. rewrite -signal_spec right_id assoc sep_elim_l comm.
+      apply sep_mono_r. rewrite /y_inv -(exist_intro (λ: "z", "z" + '42)%L).
+      apply sep_intro_True_r; first done. apply: always_intro.
+      apply forall_intro=>n. wp_let. wp_op. by apply const_intro. }
+    (* The two spawned threads, the waiters. *)
+    ewp eapply recv_split. rewrite comm. apply sep_mono.
+    { apply recv_mono. rewrite y_inv_split. done. }
+    apply wand_intro_r. wp_seq. ewp eapply wp_fork.
+    rewrite [heap_ctx _]always_sep_dup !assoc [(_ ★ recv _ _ _ _)%I]comm.
+    rewrite -!assoc assoc. apply sep_mono.
+    - wp_seq. by rewrite -worker_safe comm.
+    - by rewrite -worker_safe.
   Qed.
 End client.
 
